ral
git-svn-id: svn://scm.gforge.inria.fr/svn/cfml@47 ba02c806-7d2b-4818-9a48-35b22e6bdc79

okasaki/AltBinaryRandomAccessList.ml
@@ -1,7 +1,7 @@
 open Okasaki
 open RandomAccessListSig
 
-module AltBinaryRandomAccesList : RandomAccessList =
+module AltBinaryRandomAccessList : RandomAccessList =
 struct
 
    (* todo: name conflict with Nil *)
