okasaki/BinaryRandomAccessList_proof.v
@@ -1,0 +1,141 @@
+Set Implicit Arguments. 
+Require Import FuncTactics LibCore.
+Require Import RandomAccessListSig_ml RandomAccessListSig_proof.
+Require Import BinaryRandomAccessList_ml.
+
+Module BinaryRandomAccessListSpec <: RandomAccessListSigSpec.
+
+(** instantiations *)
+
+Module Import C <: MLRandomAccessList := MLBinaryRandomAccessList. 
+Import MLAltBinaryRandomAccesList.
+
+(** invariant *)
+
+Inductive btree : int -> tree -> multiset T -> Prop :=
+  | btree_nil : forall x X,
+      rep x X ->
+      btree 0 (Node 0 x nil) \{X}
+  | btree_cons : forall r r' x X t ts E Es E',
+      rep x X ->
+      btree r t E ->
+      btree r (Node r x ts) Es ->
+      foreach (is_ge X) E' -> 
+      r' =' r+1 ->
+      E' =' E \u Es ->
+      btree r' (Node r' x (t::ts)) E'.
+
+Inductive inv : int -> heap -> multiset T -> Prop :=
+  | inv_nil : forall r,
+      0 <= r -> inv r nil \{} 
+  | inv_node : forall rs r r' t ts E Es E',
+      btree r t E ->
+      inv rs ts Es ->
+      0 <= r' ->
+      r' <= r ->
+      r < rs ->
+      E' =' E \u Es ->
+      inv r' (t::ts) E'.
+
+Fixpoint size (t:tree) : nat :=
+  let '(Node r x ts) := t in 
+  (1 + List.fold_right (fun t x => (x + size t)%nat) 0%nat ts)%nat.
+
+Lemma size_pos : forall t, size t > 0%nat.
+Proof. destruct t. simpl. math. Qed.
+
+Lemma btree_unique : forall t n1 n2 E1 E2, 
+  btree n1 t E1 -> btree n2 t E2 -> E1 = E2.
+Proof. 
+  intros t. gen_eq m: (size t). gen t.
+  induction m using peano_induction.
+  introv M HX HY. subst m.
+  inverts HX; inverts HY. prove_rep.
+  maths (r = r0). subst. fequals.
+  applys* H. simpl; math.
+  applys* H. simpl. forwards: (size_pos t0). math.
+Qed.
+
+Hint Resolve btree_unique : rep.
+
+Global Instance heap_rep : Rep heap (multiset T).
+Proof.
+  apply (Build_Rep (inv 0)). intros x.
+  set (n:=0) at 1. generalize 0. subst n. generalize 0.
+  induction x; introv HX HY; inverts HX; inverts HY; subst; prove_rep.
+Defined.
+
+Global Instance queue_rep `{Rep a A} : Rep (queue a) (list A).
+Proof. intros. apply (Build_Rep (
+  fun (q:queue a) (Q:list A) =>
+  let (f,r) := q in 
+     Forall2 rep (f ++ rev r) Q
+  /\ (f = nil -> r = nil))).
+  destruct x; introv [? ?] [? ?].
+  asserts: (rep (l++rev l0) X). auto~.
+  asserts: (rep (l++rev l0) Y). auto~.
+  prove_rep. (* todo: improve *)
+Defined.
+
+(** automation *)
+
+Hint Constructors Forall2.
+Hint Resolve Forall2_last.
+Hint Extern 1 (@rep (rlist _) _ _ _ _) => simpl.
+Ltac auto_tilde ::= eauto.
+
+(** useful facts *)
+
+(** verification *)
+
+Section Polymorphic.
+Variables (a A : Type) (RA:Rep a A).
+
+Lemma empty_spec : 
+  rep (@empty a) (@nil A).
+Proof.
+  generalizes RA A. apply (empty_cf a). xgo.
+  intros. simpl. rew_list~. 
+Qed.
+
+Lemma is_empty_spec : 
+  RepTotal is_empty (L;rlist a) >> bool_of (L = nil).
+Proof.
+  xcf. intros (f0,r0) l [H M]. xgo.
+  rewrite~ M in H. inverts~ H.
+  intro_subst_hyp. inverts H as K.
+   destruct (nil_eq_app_rev_inv K). false.
+Qed.
+
+Lemma cons_spec : 
+  RepTotal cons (X;a) (L;rlist a) >> (X::L) ; rlist a.
+Proof.
+Qed.
+
+Lemma head_spec : 
+  RepSpec head (L;rlist a) |R>>
+     L <> nil -> R (is_head L ;; a).
+Proof.
+Qed.
+
+Lemma tail_spec :
+  RepSpec tail (L;rlist a) |R>> 
+     L <> nil -> R (is_tail L ;; rlist a).
+Proof.
+Qed.
+
+Lemma lookup_spec : 
+  RepSpec lookup (i;int) (L;rlist a) |R>>
+     0 <= i -> i < length L -> R (Nth (abs i) L ;; a).
+Proof.
+Qed.
+
+Lemma update_spec :
+  RepSpec update (i;int) (X;a) (L;rlist a) |R>> 
+     0 <= i -> i < length L -> R (Update (abs i) X L ;; rlist a).
+Proof.
+Qed.
+
+End Polymorphic.
+
+End BatchedQueueSpec.
